\documentclass[11pt]{article}
\usepackage{amsmath, amssymb, amsthm}
\usepackage[retainorgcmds]{IEEEtrantools}

\usepackage{tikz}

\usepackage{fancyhdr}

%Format stuff
\pagestyle{fancy}
\headheight 35pt

%Header info
\chead{\Large \textbf{Loaded String and Wave Equation}}
\lhead{}
\rhead{}

\begin{document}
\section{Loaded String}
	The loaded string is fundamentally equivalent to an n-oscillator system, but normal modes are much easier to visualize when masses are displaced vertically in this system.
	\begin{center}
	\begin{tikzpicture}
		[scale=1,line cap=round,
		%Styles
		axes/.style=,
		important line/.style={very thick},
		information text/.style={rounded corners,fill=red!10,inner sep=1ex},
		dot/.style={circle,inner sep=1pt,fill,label={#1},name=#1}			
		]
		
		%Colors
		\colorlet{anglecolor}{green!50!black}	%angle arcs/lines
		
		%The graphic
		\draw[color=black,very thick] (0, -1.5) -- (0, 1.5);
		\draw[color=black,very thick] (8, -1.5) -- (8, 1.5);
		\foreach \i in {.5,1.5,...,7.5}
		{
			\draw[color=orange,thick] (\i - .2, 0) -- +(-.3, 0);
			\filldraw[color=blue!20,draw=blue] (\i, 0) circle (.2);
			\draw[color=orange,thick] (\i + .2, 0) -- +(.3,0);
		}
		
		\node[above=3pt,black,font=\footnotesize] at (.5, 0) {$m_1$};
		\node[above=3pt,black,font=\footnotesize] at (7.5,0) {$m_n$};
		
		\draw (.5, -.55) -- (.5, -.85);
		\draw (1.5, -.55) -- (1.5, -.85);
		\draw[<->] (.5, -.7) -- node[below] {$l$} (1.5, -.7);
	\end{tikzpicture}
	\end{center}
	
	If each mass in the system is displaced vertically a random amount, the free-body diagram for an arbitrary mass $m_p$ in the system looks like:
		\begin{center}
		\begin{tikzpicture}
			[scale=1,line cap=round,
			%Styles
			axes/.style=,
			important line/.style={very thick},
			information text/.style={rounded corners,fill=red!10,inner sep=1ex},
			dot/.style={circle,inner sep=2pt,fill,label={#1},name=#1}			
			]
			
			%Colors
			\colorlet{anglecolor}{green!50!black}	%angle arcs/lines
			
			%The graphic
			\draw[thick,->] (0,0) -- (0, 3.5);
			\draw[thick,->] (0,0) -- (8, 0);
			
			\draw[blue,thick] (3.75, 1.25) rectangle (4.25, 1.75);
			\draw[<-,thick,orange] (4, 1.5) -- node[above,black] {$T$} (6, 3);
			\draw[->,thick,orange] (4, 1.5) -- node[above,black] {$T$} (2, 1);
			
			\node[dot=$m_{p+1}$] at (6, 3) {};
			\node[dot=$m_{p-1}$] at (2, 1) {};
			
			\draw[dashed,green!70!black] (2, 1) -- (4, 1) -- (4, 1.5) -- (6, 1.5) -- (6, 3);
			\draw[ultra thick] (-.1, 1) node[left] {$y_{p-1}$} -- (.1, 1);
			\draw[ultra thick] (-.1, 1.5) node[left] {$y_p$} -- (.1, 1.5);
			\draw[ultra thick] (-.1, 3) node[left] {$y_{p+1}$} -- (.1, 3);
		\end{tikzpicture}
		\end{center}
		
	\subsection{Equation of Motion}
		\begin{equation}
			F_{y}^{(p)} = -T\sin(\alpha_{p-1}) + T\sin(\alpha_{p+1})
		\end{equation}
		Assuming small oscillations simplifies the calculation quite a bit.
		\begin{IEEEeqnarray}{rCl}
			\sin(\alpha_{p-1}) & \approx & \frac{y_p - y_{p-1}}{l}\\
			\sin(\alpha_{p+1}) & \approx & \frac{y_{p+1} - y_p}{l}
		\end{IEEEeqnarray}
		\begin{IEEEeqnarray}{rCl}
			-\frac{T}{l} (y_p - y_{p-1}) + \frac{T}{l}(y_{p+1} - y_p) & = & m\ddot{y}_p\\
			\ddot{y}_p + \frac{T}{ml}(2y_p) - \frac{T}{ml}y_{p-1} - \frac{T}{ml}y_{p+1} & = & 0
		\end{IEEEeqnarray}
		For the loaded string, set the natural frequency
		\begin{equation}
			\omega_0^2 = \frac{T}{ml}
		\end{equation}
		Which gives
		\begin{equation}
			\ddot{y}_p + 2\omega_0^2 y_p - \omega_0^2 (y_{p+1} + y_{p-1}) = 0
		\end{equation}
		
	\subsection{Normal Modes}
		Making the assumption that the normal modes are in the form 
		\begin{equation}
			y_p = A_p e^{i\omega t}
		\end{equation}
		after substitution the following set of solutions is obtained.
		\begin{IEEEeqnarray}{rCl}
			y_p & = & c\sin(p\theta)e^{i\omega_p t}\\
			\omega_n & = & 2\omega_0 \sin\left(\frac{\theta}{2}\right)\\
			\theta & = & \frac{n\pi}{N+1}
		\end{IEEEeqnarray}
		
		Also, the relationship between adjacent amplitudes is
		\begin{equation}
			\frac{A_{p-1} + A_{p+1}}{A_p} = \frac{-\omega^2 + 2\omega_0^2}{\omega_0^2}
		\end{equation}
		
		In this equation, $p$ is an integer pointing to one of the masses in the system, and $N$ is the total number of masses. $n$ denotes which normal mode that the equation describes. There are $N$ different total normal modes in the system because the time evolution and amplitude are both periodic functions.
		
	\subsection{General Solution}
		Just like the general solution to the coupled mechanical oscillators, the position of any one particle is a combination of normal modes.
		\begin{equation}
			y_p = \sum_{n=1}^N c_n \sin\left(\frac{n\pi}{N+1}\right) e^{i\omega_n t}
		\end{equation}
		Define the eigenvectors of each normal mode as
		\begin{equation}
			\mathbf{q_n} = \left( \sin \left(\frac{n\pi}{N+1}\right), \sin \left(\frac{2n\pi}{N+1}\right), \ldots , \sin \left(\frac{Nn\pi}{N+1}\right) \right)
		\end{equation}
		This gives the general solution to all the masses:
		\begin{equation}
			\mathbf{y} = \sum_{n=1}^N a_n \mathbf{q_n} e^{i\omega_n t}
		\end{equation}
		
		\subparagraph{Initial Conditions} Just like the 2 coupled mechanical oscillators, the real and imaginary coefficients for the complex coefficient are given by 
			\begin{equation}
				a_n = \frac{\mathbf{x_0} \cdot \mathbf{q_n}}{|\mathbf{q_n}|^2}
			\end{equation}
			\begin{equation}
				b_n = \frac{-\mathbf{v_0} \cdot \mathbf{q_n}}{\omega_n |\mathbf{q_n}|^2}
			\end{equation}
		
\section{Wave Equation}
	If $N$ is taken to $\infty$, then $l$ goes to 0. In this case, the loaded string becomes something more like a continuous rope or wave. Consider the original equation of motion:
	\begin{equation}
		\ddot{y}_p + 2\omega_0^2 y_p - \omega_0^2(y_{p+1} + y_{p-1}) - 0
	\end{equation}
	Rearrange the equation and substitute $\omega_0^2 = T/ml$.
	\begin{IEEEeqnarray}{rCl}
		m\ddot{y}_p & = & \frac{T}{l}(y_{p+1} - y_p) - \frac{T}{l}(y_p - y_{p-1})\\
		\frac{m\ddot{y}_p}{l} & = & \frac{T}{l} \left( \frac{y_{p+1} - y_p}{l} \right) - \frac{T}{l}\left( \frac{y_p - y_{p-1}}{l} \right)
	\end{IEEEeqnarray}
	
	Now define $\rho = m/l$ as the \textbf{mass density} of the system. Note that as $l$ approaches 0,
	\begin{equation}
		\frac{y_{p+1} - y_p}{l} = \left.\frac{dy}{dx}\right|_{x + l/2}
	\end{equation}
	\begin{equation}
		\frac{y_p - y_{p-1}}{l} = \left.\frac{dy}{dx}\right|_{x - l/2}
	\end{equation}
	Because of the $l$ in the denominator for the coefficients of both of these derivatives, the right hand side of the equation is actually a second derivative:
	
	\begin{center}
	\begin{tikzpicture}
		[scale=1,line cap=round,
		%Styles
		axes/.style=,
		important line/.style={very thick},
		information text/.style={rounded corners,fill=red!10,inner sep=1ex},
		dot/.style={circle,inner sep=1pt,fill,label={#1},name=#1}			
		]
		
		%Colors
		\colorlet{anglecolor}{green!50!black}	%angle arcs/lines
		
		%The graphic
		\draw[<->,thick] (0, 3) -- (0, 0) -- (3.5, 0);
		\foreach \i in {1,...,3}
		{
			\draw[ultra thick] (\i, .1) -- (\i, -.1);
		}
		\node[below] at (1, -.1) {$x - \frac{l}{2}$};
		\node[below] at (2, -.1) {$x$};
		\node[below] at (3, -.1) {$x + \frac{l}{2}$};
		
		\node[below] at (3.5,0) {$x$};
		\node[left] at (0, 3) {$\frac{dy}{dx}$};
		
		\filldraw (1,1.5) circle (.05);
		\filldraw (3,2.5) circle (.05);
		
		\draw[blue,thick] (1,1.5) -- node[black,above left] {$\frac{d^2 y}{dx^2}$}(3,2.5);
		\draw[dashed,orange] (3,2.5) -- (3,1.5) -- node[below,black] {$l$} (1, 1.5);
	\end{tikzpicture}
	\end{center}
	This leads to the \textbf{wave equation}:
	\begin{equation}
		\rho \ddot{y} = T \cdot \frac{d^2 y}{dx^2}
	\end{equation}
	
	\subsection{Normal Modes}
		Let $y^{(n)}(t, x)$ denote the n-th normal mode for the continuous system.
		\begin{IEEEeqnarray}{rCl}
			y^{(n)}(t,x) & = & c_n \sin\left( \frac{n\pi x}{L} \right)e^{i\omega_n t}\\
			\omega_n & = & \frac{n\pi}{L} \sqrt{\frac{T}{\rho}}
		\end{IEEEeqnarray}
		The expression for $\omega_n$ only holds for small oscillations, based on the observation that $\sin\theta \approx \theta$ for small values of $\theta$.
		
		The general solution is a superposition of all normal modes.
		\begin{equation}
			y(t, x) = \sum_{n=1}^\infty c_n \sin\left( \frac{n\pi x}{L} \right)e^{i\omega_n t}
		\end{equation}
		
	\subsection{Initial Conditions}
		Take the following initial conditions:
		\begin{IEEEeqnarray}{rCl}
			y(x, t=0) & = & \sum_0^\infty a_n \sin\left( \frac{n\pi x}{L} \right)\\
			\dot{y}(x, t=0) & = & \sum_0^\infty -\omega_n b_n \sin\left( \frac{n\pi x}{L} \right)
		\end{IEEEeqnarray}
		Remember that the normal mode eigenvectors are all orthogonal to each other. In the continuous case, when there are an infinite number of terms in the eigenvectors, the statement of orthogonality follows \textbf{Foiurier's Trick}, which states that
		\begin{equation}
			\int_0^L \sin\left( \frac{n\pi x}{L} \right) \sin\left( \frac{m\pi x}{L} \right) dx = \frac{L}{2}\delta_{nm}
		\end{equation}
		Note that this is simply the dot product of two normal mode eigenvectors generalized to an infinite number of terms.
		
		From this property, it is trivial to show that
		\begin{equation}
			\int_0^L \sin\left( \frac{n\pi x}{L} \right) y(x, t=0)dx = a_n \frac{L}{2}
		\end{equation}
		
		Therefore, for any initial conditions $y(x, t=0)$ and $\dot{y}(x, t=0)$, the real and imaginary parts of the normal mode coefficients can be derived with
		\begin{IEEEeqnarray}{rCl}
			a_n & = & \frac{2}{L} \int_0^L \sin\left( \frac{n\pi x}{L} \right) y(x, t=0)dx\\
			b_n & = & \frac{-2}{\omega_n L} \int_0^L \sin\left( \frac{n\pi x}{L} \right) \dot{y}(x, t=0)dx
		\end{IEEEeqnarray}

%	\begin{center}
%	\begin{tikzpicture}
%		[scale=3,line cap=round,
%		%Styles
%		axes/.style=,
%		important line/.style={very thick},
%		information text/.style={rounded corners,fill=red!10,inner sep=1ex},
%		dot/.style={circle,inner sep=1pt,fill,label={#1},name=#1}			
%		]
%		
%		%Colors
%		\colorlet{anglecolor}{green!50!black}	%angle arcs/lines
%		
%		%The graphic
%	\end{tikzpicture}
%	\end{center}

%	\begin{figure}[htb]
%		\centering
%		\includegraphics[width=0.8\textwidth]{filename.eps}
%		\caption{Caption.}
%		\label{fig:figure}
%	\end{figure}

%		\def\enotesize{\normalsize}
%		\theendnotes
\end{document}